src/program_proof/tulip/program/gcoord/group_coordinator.v
@@ -1,0 +1,811 @@
+From Perennial.program_proof.tulip.invariance Require Import read.
+From Perennial.program_proof.tulip.program Require Import prelude.
+From Perennial.program_proof.tulip.program Require Import prelude group_reader group_preparer.
+
+Section repr.
+  Context `{!heapGS Σ, !tulip_ghostG Σ}.
+
+  (*@ type GroupCoordinator struct {                                          @*)
+  (*@     // Replica addresses. Read-only.                                    @*)
+  (*@     rps     map[uint64]grove_ffi.Address                                @*)
+  (*@     // Mutex protecting fields below.                                   @*)
+  (*@     mu      *sync.Mutex                                                 @*)
+  (*@     // Condition variable used to notify arrival of responses.          @*)
+  (*@     cv      *sync.Cond                                                  @*)
+  (*@     // Timestamp of the currently active transaction.                   @*)
+  (*@     ts       uint64                                                     @*)
+  (*@     // ID of the replica believed to be the leader of this group.       @*)
+  (*@     leader   uint64                                                     @*)
+  (*@     // Group reader.                                                    @*)
+  (*@     grd      *GroupReader                                               @*)
+  (*@     // Group preparer.                                                  @*)
+  (*@     gpp      *GroupPreparer                                             @*)
+  (*@     // IDs of the finalizing transactions. Using unit as range would suffice. @*)
+  (*@     tsfinals map[uint64]bool                                            @*)
+  (*@     // Connections to replicas.                                         @*)
+  (*@     conns    map[uint64]grove_ffi.Connection                            @*)
+  (*@ }                                                                       @*)
+  Definition own_gcoord_ts gcoord ts : iProp Σ :=
+    ∃ (tsW : u64),
+      "HtsW" ∷ gcoord ↦[GroupCoordinator :: "ts"] #tsW ∗
+      "%Hts" ∷ ⌜uint.nat tsW = ts⌝.
+
+  Definition own_gcoord_greader gcoord ts γ : iProp Σ :=
+    ∃ (grdP : loc),
+      "HgrdP" ∷ gcoord ↦[GroupCoordinator :: "grd"] #grdP ∗
+      "Hgrd"  ∷ own_greader grdP ts γ.
+
+  Definition own_gcoord_gpreparer gcoord ts gid γ : iProp Σ :=
+    ∃ (gppP : loc),
+      "HgppP" ∷ gcoord ↦[GroupCoordinator :: "gpp"] #gppP ∗
+      "Hgpp"  ∷ own_gpreparer gppP ts gid γ.
+
+  Definition own_gcoord_finalizer gcoord : iProp Σ :=
+    ∃ (leader : u64) (tsfinalsP : loc) (tsfinals : gmap u64 bool),
+      "Hleader"    ∷ gcoord ↦[GroupCoordinator :: "leader"] #leader ∗
+      "HtsfinalsP" ∷ gcoord ↦[GroupCoordinator :: "tsfinals"] #tsfinalsP ∗
+      "Htsfinals"  ∷ own_map tsfinalsP DfracDiscarded tsfinals.
+
+  Definition own_gcoord_core gcoord ts gid γ : iProp Σ :=
+    "Hts" ∷ own_gcoord_ts gcoord ts ∗
+    "Hgrd" ∷ own_gcoord_greader gcoord ts γ ∗
+    "Hgpp" ∷ own_gcoord_gpreparer gcoord ts gid γ ∗
+    "Hgfl" ∷ own_gcoord_finalizer gcoord.
+
+  Definition own_gcoord_comm gcoord (rps : gmap u64 chan) : iProp Σ :=
+    ∃ (connsP : loc) (conns : gmap u64 (chan * chan)),
+      let connsV := fmap (λ x, connection_socket x.1 x.2) conns in
+      "HconnsP" ∷ gcoord ↦[GroupCoordinator :: "conns"] #connsP ∗
+      "Hconns"  ∷ map.own_map connsP (DfracOwn 1) (connsV, #()) ∗
+      (* "#Htrmls" ∷ ([∗ map] x ∈ conns, is_terminal γ x.1) ∗ *)
+      "%Haddrpeers" ∷ ⌜map_Forall (λ rid x, rps !! rid = Some x.2) conns⌝.
+
+  Definition own_gcoord_with_ts gcoord rps ts gid γ : iProp Σ :=
+    "Hgcoord" ∷ own_gcoord_core gcoord ts gid γ ∗
+    "Hcomm"   ∷ own_gcoord_comm gcoord rps.
+
+  Definition own_gcoord gcoord rps gid γ : iProp Σ :=
+    ∃ ts, "Hgcoord" ∷ own_gcoord_with_ts gcoord rps ts gid γ.
+
+  Definition is_gcoord_rps gcoord (rps : gmap u64 chan) : iProp Σ :=
+    ∃ (rpsP : loc),
+      "HrpsP" ∷ readonly (gcoord ↦[GroupCoordinator :: "rps"] #rpsP) ∗
+      "#Hrps" ∷ own_map rpsP DfracDiscarded rps.
+
+  Definition is_gcoord_with_rps gcoord gid (rps : gmap u64 chan) γ : iProp Σ :=
+    ∃ (muP : loc) (cvP : loc),
+      "#HmuP"  ∷ readonly (gcoord ↦[GroupCoordinator :: "mu"] #muP) ∗
+      "#Hlock" ∷ is_lock tulipNS #muP (own_gcoord gcoord rps gid γ) ∗
+      "#HcvP"  ∷ readonly (gcoord ↦[GroupCoordinator :: "cv"] #cvP) ∗
+      "Hcv"    ∷ is_cond cvP #muP ∗
+      "#Hrps"  ∷ is_gcoord_rps gcoord rps.
+
+  Definition is_gcoord gcoord gid γ : iProp Σ :=
+    ∃ rps, "Hgcoord" ∷ is_gcoord_with_rps gcoord gid rps γ.
+
+End repr.
+
+Section program.
+  Context `{!heapGS Σ, !tulip_ghostG Σ}.
+
+  Theorem wp_GroupCoordinator__attachedWith (gcoord : loc) (tsW : u64) tscur gid γ :
+    let ts := uint.nat tsW in
+    {{{ own_gcoord_core gcoord tscur gid γ }}}
+      GroupCoordinator__attachedWith #gcoord #tsW
+    {{{ (ok : bool), RET #ok;
+        if ok then own_gcoord_core gcoord ts gid γ else own_gcoord_core gcoord tscur gid γ
+    }}}.
+  Proof.
+    iIntros (ts Φ) "Hgcoord HΦ".
+    wp_rec.
+
+    (*@ func (gcoord *GroupCoordinator) attachedWith(ts uint64) bool {          @*)
+    (*@     return gcoord.ts == ts                                              @*)
+    (*@ }                                                                       @*)
+    iNamed "Hgcoord".
+    rename tsW into tsargW. iNamed "Hts".
+    wp_loadField.
+    wp_pures.
+    case_bool_decide as Htsarg.
+    { iApply "HΦ". inv Htsarg. by iFrame "∗ # %". }
+    { iApply "HΦ". by iFrame "∗ # %". }
+  Qed.
+
+  Theorem wp_GroupCoordinator__AttachedWith (gcoord : loc) (ts : u64) gid γ :
+    is_gcoord gcoord gid γ -∗
+    {{{ True }}}
+      GroupCoordinator__AttachedWith #gcoord #ts
+    {{{ (attached : bool), RET #attached; True }}}.
+  Proof.
+    iIntros "#Hgcoord" (Φ) "!> _ HΦ".
+    wp_rec.
+
+    (*@ func (gcoord *GroupCoordinator) AttachedWith(ts uint64) bool {          @*)
+    (*@     gcoord.mu.Lock()                                                    @*)
+    (*@     b := gcoord.attachedWith(ts)                                        @*)
+    (*@     gcoord.mu.Unlock()                                                  @*)
+    (*@     return b                                                            @*)
+    (*@ }                                                                       @*)
+    do 2 iNamed "Hgcoord".
+    wp_loadField.
+    wp_apply (wp_Mutex__Lock with "Hlock").
+    iIntros "[Hlocked Hgcoord]".
+    do 2 iNamed "Hgcoord".
+    wp_apply (wp_GroupCoordinator__attachedWith with "Hgcoord").
+    iIntros (b) "Hgcoord".
+    wp_loadField.
+    wp_apply (wp_Mutex__Unlock with "[-HΦ]").
+    { iFrame "Hlock Hlocked". by destruct b; iFrame. }
+    wp_pures.
+    by iApply "HΦ".
+  Qed.
+
+  Theorem wp_GroupCoordinator__ValueResponded gcoord (rid : u64) key gid γ :
+    is_gcoord gcoord gid γ -∗
+    {{{ True }}}
+      GroupCoordinator__ValueResponded #gcoord #rid #(LitString key)
+    {{{ (ok : bool), RET #ok; True }}}.
+  Proof.
+    iIntros "#Hgcoord" (Φ) "!> _ HΦ".
+    wp_rec.
+
+    (*@ func (gcoord *GroupCoordinator) ValueResponded(rid uint64, key string) bool { @*)
+    (*@     gcoord.mu.Lock()                                                    @*)
+    (*@     done := gcoord.grd.responded(rid, key)                              @*)
+    (*@     gcoord.mu.Unlock()                                                  @*)
+    (*@     return done                                                         @*)
+    (*@ }                                                                       @*)
+    do 2 iNamed "Hgcoord".
+    wp_loadField.
+    wp_apply (wp_Mutex__Lock with "Hlock").
+    iIntros "[Hlocked Hgcoord]".
+    do 3 iNamed "Hgcoord". iNamed "Hgrd".
+    wp_loadField.
+    wp_pures.
+    wp_apply (wp_GroupReader__responded with "Hgrd").
+    iIntros (responded) "Hgrd".
+    wp_loadField.
+    wp_apply (wp_Mutex__Unlock with "[-HΦ]").
+    { iFrame "Hlock Hlocked". by iFrame "∗ # %". }
+    wp_pures.
+    by iApply "HΦ".
+  Qed.
+
+  Theorem wp_GroupCoordinator__WaitUntilValueReady
+    (gcoord : loc) (tsW : u64) (key : string) gid γ :
+    let ts := uint.nat tsW in
+    is_gcoord gcoord gid γ -∗
+    {{{ True }}}
+      GroupCoordinator__WaitUntilValueReady #gcoord #tsW #(LitString key)
+    {{{ (value : dbval) (valid : bool), RET (dbval_to_val value, #valid); 
+        if valid then fast_or_quorum_read γ key ts value else True
+    }}}.
+  Proof.
+    iIntros (ts) "#Hgcoord".
+    iIntros (Φ) "!> _ HΦ".
+    wp_rec.
+
+    (*@ func (gcoord *GroupCoordinator) WaitUntilValueReady(ts uint64, key string) (tulip.Value, bool) { @*)
+    (*@     var value tulip.Value                                               @*)
+    (*@     var valid bool                                                      @*)
+    (*@                                                                         @*)
+    wp_apply wp_ref_of_zero; first done.
+    iIntros (valueP) "HvalueP".
+    wp_apply wp_ref_of_zero; first done.
+    iIntros (validP) "HvalidP".
+
+    (*@     gcoord.mu.Lock()                                                    @*)
+    (*@                                                                         @*)
+    do 2 iNamed "Hgcoord".
+    wp_loadField.
+    wp_apply (wp_Mutex__Lock with "Hlock").
+    iIntros "[Hlocked Hgcoord]".
+    wp_pures.
+
+    (*@     for {                                                               @*)
+    (*@                                                                         @*)
+    set P := (λ (cont : bool), ∃ (value : dbval) (valid : bool),
+      "Hgcoord" ∷ own_gcoord gcoord rps gid γ ∗
+      "HvalueP" ∷ valueP ↦[boolT * (stringT * unitT)%ht] dbval_to_val value ∗
+      "HvalidP" ∷ validP ↦[boolT] #valid ∗
+      "Hlocked" ∷ locked #muP ∗
+      "#Hread"  ∷ if (negb cont) && valid then fast_or_quorum_read γ key ts value else True)%I.
+    wp_apply (wp_forBreak P with "[] [Hgcoord HvalueP HvalidP Hlocked]"); last first; first 1 last.
+    { iFrame. by iExists None. }
+    { clear Φ.
+
+      (*@         if !gcoord.attachedWith(ts) {                                   @*)
+      (*@             valid = false                                               @*)
+      (*@             break                                                       @*)
+      (*@         }                                                               @*)
+      (*@                                                                         @*)
+      iIntros (Φ) "!> HP HΦ".
+      iNamed "HP".
+      iDestruct"Hgcoord" as (tscur) "Hgcoord".
+      do 2 iNamed "Hgcoord".
+      wp_apply (wp_GroupCoordinator__attachedWith with "Hgcoord").
+      iIntros (attached) "Hgcoord".
+      wp_pures.
+      destruct attached; wp_pures; last first.
+      { wp_store. iApply "HΦ". by iFrame. }
+
+      (*@         v, ok := gcoord.grd.read(key)                                   @*)
+      (*@         if ok {                                                         @*)
+      (*@             value = v                                                   @*)
+      (*@             valid = true                                                @*)
+      (*@             break                                                       @*)
+      (*@         }                                                               @*)
+      (*@                                                                         @*)
+      iNamed "Hgcoord". iNamed "Hgrd".
+      wp_loadField.
+      wp_apply (wp_GroupReader__read with "Hgrd").
+      iIntros (v ok) "[Hgrd #Hreadv]".
+      wp_pures.
+      destruct ok; wp_pures.
+      { wp_apply (wp_StoreAt with "HvalueP").
+        { by destruct v; auto. }
+        iIntros "HvalueP".
+        wp_store.
+        iApply "HΦ".
+        by iFrame "∗ #".
+      }
+    
+      (*@         gcoord.cv.Wait()                                                @*)
+      (*@     }                                                                   @*)
+      (*@                                                                         @*)
+      wp_loadField.
+      wp_apply (wp_Cond__Wait with "[-HΦ HvalueP HvalidP]").
+      { by iFrame "Hcv Hlock Hlocked ∗ # %". }
+      iIntros "[Hlocked Hgcoord]".
+      wp_pures.
+      iApply "HΦ".
+      by iFrame.
+    }
+    subst P. iNamed 1.
+
+    (*@     gcoord.mu.Unlock()                                                  @*)
+    (*@                                                                         @*)
+    wp_loadField.
+    wp_apply (wp_Mutex__Unlock with "[-HΦ HvalueP HvalidP]").
+    { by iFrame "Hlock Hlocked Hgcoord". }
+
+    (*@     return value, valid                                                 @*)
+    (*@ }                                                                       @*)
+    do 2 wp_load.
+    wp_pures.
+    iApply "HΦ".
+    by destruct valid.
+  Qed.
+
+  Theorem wp_GroupCoordinator__SendRead
+    (gcoord : loc) (rid : u64) (ts : u64) (key : string) gid γ :
+    is_gcoord gcoord gid γ -∗
+    {{{ True }}}
+      GroupCoordinator__SendRead #gcoord #rid #ts #(LitString key)
+    {{{ RET #(); True }}}.
+  Proof.
+    (*@ func (gcoord *GroupCoordinator) SendRead(rid, ts uint64, key string) {  @*)
+    (*@     gcoord.Send(rid, message.EncodeTxnRead(ts, key))                    @*)
+    (*@ }                                                                       @*)
+  Admitted.
+
+  Theorem wp_GroupCoordinator__ReadSession 
+    (gcoord : loc) (rid : u64) (ts : u64) (key : string) gid γ :
+    is_gcoord gcoord gid γ -∗
+    {{{ True }}}
+      GroupCoordinator__ReadSession #gcoord #rid #ts #(LitString key)
+    {{{ RET #(); True }}}.
+  Proof.
+    iIntros "#Hgcoord" (Φ) "!> _ HΦ".
+    wp_rec.
+
+    (*@ func (gcoord *GroupCoordinator) ReadSession(rid uint64, ts uint64, key string) { @*)
+    (*@     for !gcoord.ValueResponded(rid, key) && gcoord.AttachedWith(ts) {   @*)
+    (*@         gcoord.SendRead(rid, ts, key)                                   @*)
+    (*@         primitive.Sleep(params.NS_RESEND_READ)                          @*)
+    (*@     }                                                                   @*)
+    (*@                                                                         @*)
+    wp_pures.
+    wp_apply (wp_forBreak_cond (λ _, True)%I with "[] []"); last first; first 1 last.
+    { done. }
+    { clear Φ.
+      iIntros (Φ) "!> _ HΦ".
+      wp_apply (wp_GroupCoordinator__ValueResponded with "Hgcoord").
+      iIntros (resped) "_".
+      wp_pures.
+      destruct resped; wp_pures.
+      { by iApply "HΦ". }
+      wp_apply (wp_GroupCoordinator__AttachedWith with "Hgcoord").
+      iIntros (attached) "_".
+      destruct attached; wp_pures; last first.
+      { by iApply "HΦ". }
+      wp_apply (wp_GroupCoordinator__SendRead with "Hgcoord").
+      wp_apply wp_Sleep.
+      wp_pures.
+      by iApply "HΦ".
+    }
+
+    (*@     // Either replica @rid has already responded with its value, or the value @*)
+    (*@     // for @key has already been determined. In either case, the corresponding @*)
+    (*@     // read session could terminate.                                    @*)
+    (*@ }                                                                       @*)
+    wp_pures.
+    by iApply "HΦ".
+  Qed.
+
+  Theorem wp_GroupCoordinator__Read
+    (gcoord : loc) (tsW : u64) (key : string) gid γ :
+    let ts := uint.nat tsW in
+    is_gcoord gcoord gid γ -∗
+    {{{ True }}}
+      GroupCoordinator__Read #gcoord #tsW #(LitString key)
+    {{{ (value : dbval) (ok : bool), RET (dbval_to_val value, #ok); 
+        if ok then fast_or_quorum_read γ key ts value else True
+    }}}.
+  Proof.
+    iIntros (ts) "#Hgcoord".
+    iIntros (Φ) "!> _ HΦ".
+    wp_rec.
+
+    (*@ func (gcoord *GroupCoordinator) Read(ts uint64, key string) (tulip.Value, bool) { @*)
+    (*@     // Spawn a session with each replica in the group.                  @*)
+    (*@     for ridloop := range(gcoord.rps) {                                  @*)
+    (*@         rid := ridloop                                                  @*)
+    (*@         go func() {                                                     @*)
+    (*@             gcoord.ReadSession(rid, ts, key)                            @*)
+    (*@         }()                                                             @*)
+    (*@     }                                                                   @*)
+    (*@                                                                         @*)
+    iPoseProof "Hgcoord" as "Hgcoord'".
+    do 2 iNamed "Hgcoord". iNamed "Hrps".
+    iRename "Hgcoord'" into "Hgcoord".
+    wp_loadField.
+    wp_apply (wp_MapIter_fold _ _ _ (λ _, True)%I with "Hrps []").
+    { done. }
+    { clear Φ.
+      iIntros (mx rid c Φ) "!> _ HΦ".
+      wp_pures.
+      wp_apply wp_fork.
+      { by wp_apply (wp_GroupCoordinator__ReadSession with "Hgcoord"). }
+      by iApply "HΦ".
+    }
+    iIntros "_".
+
+    (*@     v, ok := gcoord.WaitUntilValueReady(ts, key)                        @*)
+    (*@     return v, ok                                                        @*)
+    (*@ }                                                                       @*)
+    wp_apply (wp_GroupCoordinator__WaitUntilValueReady with "Hgcoord").
+    iIntros (v ok) "#Hread".
+    wp_pures.
+    by iApply "HΦ".
+  Qed.
+
+  Theorem wp_GroupCoordinator__NextPrepareAction
+    (gcoord : loc) (rid : u64) (tsW : u64) gid γ :
+    let ts := uint.nat tsW in
+    is_gcoord gcoord gid γ -∗
+    {{{ True }}}
+      GroupCoordinator__NextPrepareAction #gcoord #rid #tsW
+    {{{ (action : gppaction) (ok : bool), RET (#(gppaction_to_u64 action), #ok); 
+        if ok then safe_gppaction γ ts gid action else True
+    }}}.
+  Proof.
+    iIntros (ts) "#Hgcoord".
+    iIntros (Φ) "!> _ HΦ".
+    wp_rec.
+
+    (*@ func (gcoord *GroupCoordinator) NextPrepareAction(rid uint64, ts uint64) (uint64, bool) { @*)
+    (*@     gcoord.mu.Lock()                                                    @*)
+    (*@                                                                         @*)
+    do 2 iNamed "Hgcoord".
+    wp_loadField.
+    wp_apply (wp_Mutex__Lock with "Hlock").
+    iIntros "[Hlocked Hgcoord]".
+    do 2 iNamed "Hgcoord".
+    wp_apply (wp_GroupCoordinator__attachedWith with "Hgcoord").
+    iIntros (ok) "Hgcoord".
+    wp_pures.
+
+    (*@     if !gcoord.attachedWith(ts) {                                       @*)
+    (*@         gcoord.mu.Unlock()                                              @*)
+    (*@         return 0, false                                                 @*)
+    (*@     }                                                                   @*)
+    (*@                                                                         @*)
+    destruct ok; wp_pures; last first.
+    { wp_loadField.
+      wp_apply (wp_Mutex__Unlock with "[-HΦ]").
+      { by iFrame "Hlock Hlocked ∗". }
+      wp_pures.
+      (* [GPPFastPrepare] just a placeholder *)
+      by iApply ("HΦ" $! GPPFastPrepare).
+    }
+
+    (*@     action := gcoord.gpp.action(rid)                                    @*)
+    (*@                                                                         @*)
+    iNamed "Hgcoord". iNamed "Hgpp".
+    wp_loadField.
+    wp_apply (wp_GroupPreparer__action with "Hgpp").
+    iIntros (action) "[Hgpp #Hsafea]".
+    wp_pures.
+
+    (*@     gcoord.mu.Unlock()                                                  @*)
+    (*@                                                                         @*)
+    wp_loadField.
+    wp_apply (wp_Mutex__Unlock with "[-HΦ]").
+    { by iFrame "Hlock Hlocked ∗". }
+
+    (*@     return action, true                                                 @*)
+    (*@ }                                                                       @*)
+    wp_pures.
+    by iApply "HΦ".
+  Qed.
+
+  Theorem wp_GroupCoordinator__WaitUntilPrepareDone
+    (gcoord : loc) (tsW : u64) gid γ :
+    let ts := uint.nat tsW in
+    is_gcoord gcoord gid γ -∗
+    {{{ True }}}
+      GroupCoordinator__WaitUntilPrepareDone #gcoord #tsW
+    {{{ (tphase : txnphase) (valid : bool), RET (#(txnphase_to_u64 tphase), #valid); 
+        if valid then safe_txnphase γ ts gid tphase else True
+    }}}.
+  Proof.
+    iIntros (ts) "#Hgcoord".
+    iIntros (Φ) "!> _ HΦ".
+    wp_rec.
+
+    (*@ func (gcoord *GroupCoordinator) WaitUntilPrepareDone(ts uint64) (uint64, bool) { @*)
+    (*@     var phase uint64                                                    @*)
+    (*@     var valid bool                                                      @*)
+    (*@                                                                         @*)
+    wp_apply wp_ref_of_zero; first done.
+    iIntros (phaseP) "HphaseP".
+    wp_apply wp_ref_of_zero; first done.
+    iIntros (validP) "HvalidP".
+
+    (*@     gcoord.mu.Lock()                                                    @*)
+    (*@                                                                         @*)
+    do 2 iNamed "Hgcoord".
+    wp_loadField.
+    wp_apply (wp_Mutex__Lock with "Hlock").
+    iIntros "[Hlocked Hgcoord]".
+    wp_pures.
+
+    (*@     for {                                                               @*)
+    (*@                                                                         @*)
+    set P := (λ (cont : bool), ∃ (pphase : gppphase) (valid : bool),
+      "Hgcoord" ∷ own_gcoord gcoord rps gid γ ∗
+      "HphaseP" ∷ phaseP ↦[uint64T] #(gppphase_to_u64 pphase) ∗
+      "HvalidP" ∷ validP ↦[boolT] #valid ∗
+      "Hlocked" ∷ locked #muP ∗
+      "#Hsafep" ∷ (if (negb cont) && valid
+                   then safe_gpreparer_phase γ ts gid pphase ∗ ⌜gpp_ready pphase⌝
+                   else True))%I.
+    wp_apply (wp_forBreak P with "[] [Hgcoord HphaseP HvalidP Hlocked]"); last first; first 1 last.
+    { iFrame. by iExists GPPValidating. }
+    { clear Φ.
+
+      (*@         if !gcoord.attachedWith(ts) {                                   @*)
+      (*@             valid = false                                               @*)
+      (*@             break                                                       @*)
+      (*@         }                                                               @*)
+      (*@                                                                         @*)
+      iIntros (Φ) "!> HP HΦ".
+      iNamed "HP".
+      iDestruct"Hgcoord" as (tscur) "Hgcoord".
+      do 2 iNamed "Hgcoord".
+      wp_apply (wp_GroupCoordinator__attachedWith with "Hgcoord").
+      iIntros (attached) "Hgcoord".
+      wp_pures.
+      destruct attached; wp_pures; last first.
+      { wp_store. iApply "HΦ". by iFrame. }
+
+      (*@         ready := gcoord.gpp.ready()                                     @*)
+      (*@         if ready {                                                      @*)
+      (*@             phase = gcoord.gpp.getPhase()                               @*)
+      (*@             valid = true                                                @*)
+      (*@             break                                                       @*)
+      (*@         }                                                               @*)
+      (*@                                                                         @*)
+      iNamed "Hgcoord". do 2 iNamed "Hgpp".
+      wp_loadField.
+      wp_apply (wp_GroupPreparer__ready_external with "Hgpp").
+      iIntros "Hgpp".
+      case_bool_decide; wp_pures.
+      { wp_loadField.
+        wp_apply (wp_GroupPreparer__getPhase with "Hgpp").
+        iIntros "[Hgpp #Hsafegpp]".
+        do 2 wp_store.
+        iApply "HΦ".
+        by iFrame "∗ # %".
+      }
+
+      (*@         gcoord.cv.Wait()                                                @*)
+      (*@     }                                                                   @*)
+      (*@                                                                         @*)
+      wp_loadField.
+      wp_apply (wp_Cond__Wait with "[-HΦ HphaseP HvalidP]").
+      { by iFrame "Hcv Hlock Hlocked ∗ # %". }
+      iIntros "[Hlocked Hgcoord]".
+      wp_pures.
+      iApply "HΦ".
+      by iFrame.
+    }
+    subst P. iNamed 1. simpl.
+
+    (*@     gcoord.mu.Unlock()                                                  @*)
+    (*@                                                                         @*)
+    wp_loadField.
+    wp_apply (wp_Mutex__Unlock with "[-HΦ HphaseP HvalidP]").
+    { by iFrame "Hlock Hlocked Hgcoord". }
+
+    (*@     if !valid {                                                         @*)
+    (*@         // TXN_PREPARED here is just a placeholder.                     @*)
+    (*@         return tulip.TXN_PREPARED, false                                @*)
+    (*@     }                                                                   @*)
+    (*@                                                                         @*)
+    wp_load. wp_pures.
+    destruct valid; wp_pures; last first.
+    { by iApply ("HΦ" $! TxnPrepared). }
+    iDestruct "Hsafep" as "[Hsafep %Hready]".
+
+    (*@     if phase == GPP_COMMITTED {                                         @*)
+    (*@         return tulip.TXN_COMMITTED, true                                @*)
+    (*@     }                                                                   @*)
+    (*@                                                                         @*)
+    wp_load. wp_pures.
+    case_bool_decide; wp_pures.
+    { iApply ("HΦ" $! TxnCommitted). by destruct pphase. }
+
+    (*@     if phase == GPP_ABORTED {                                           @*)
+    (*@         return tulip.TXN_ABORTED, true                                  @*)
+    (*@     }                                                                   @*)
+    (*@                                                                         @*)
+    wp_load. wp_pures.
+    case_bool_decide; wp_pures.
+    { iApply ("HΦ" $! TxnAborted). by destruct pphase. }
+
+    (*@     return tulip.TXN_PREPARED, true                                     @*)
+    (*@ }                                                                       @*)
+    iApply ("HΦ" $! TxnPrepared). by destruct pphase.
+  Qed.
+
+  Theorem wp_GroupCoordinator__SendFastPrepare
+    (gcoord : loc) (rid : u64) (ts : u64) (pwrsP : loc) (ptgsP : Slice.t) gid γ :
+    is_gcoord gcoord gid γ -∗
+    {{{ True }}}
+      GroupCoordinator__SendFastPrepare #gcoord #rid #ts #pwrsP (to_val ptgsP)
+    {{{ RET #(); True }}}.
+  Proof.
+    (*@ func (gcoord *GroupCoordinator) SendFastPrepare(rid, ts uint64, pwrs tulip.KVMap, ptgs []uint64) { @*)
+    (*@     gcoord.Send(rid, message.EncodeTxnFastPrepare(ts, pwrs, ptgs))      @*)
+    (*@ }                                                                       @*)
+  Admitted.
+
+  Theorem wp_GroupCoordinator__SendValidate
+    (gcoord : loc) (rid : u64) (ts : u64) (rank : u64) (pwrsP : loc) (ptgsP : Slice.t) gid γ :
+    is_gcoord gcoord gid γ -∗
+    {{{ True }}}
+      GroupCoordinator__SendValidate #gcoord #rid #ts #rank #pwrsP (to_val ptgsP)
+    {{{ RET #(); True }}}.
+  Proof.
+    (*@ func (gcoord *GroupCoordinator) SendValidate(rid, ts, rank uint64, pwrs tulip.KVMap, ptgs []uint64) { @*)
+    (*@ }                                                                       @*)
+  Admitted.
+
+  Theorem wp_GroupCoordinator__SendPrepare
+    (gcoord : loc) (rid : u64) (tsW : u64) (rank : u64) gid γ :
+    let ts := uint.nat tsW in
+    is_group_prepare_proposal γ gid ts 1%nat true -∗
+    is_gcoord gcoord gid γ -∗
+    {{{ True }}}
+      GroupCoordinator__SendPrepare #gcoord #rid #tsW #rank
+    {{{ RET #(); True }}}.
+  Proof.
+    (*@ func (gcoord *GroupCoordinator) SendPrepare(rid, ts, rank uint64) {     @*)
+    (*@ }                                                                       @*)
+  Admitted.
+
+  Theorem wp_GroupCoordinator__SendUnprepare
+    (gcoord : loc) (rid : u64) (tsW : u64) (rank : u64) gid γ :
+    let ts := uint.nat tsW in
+    is_group_prepare_proposal γ gid ts 1%nat false -∗
+    is_gcoord gcoord gid γ -∗
+    {{{ True }}}
+      GroupCoordinator__SendUnprepare #gcoord #rid #tsW #rank
+    {{{ RET #(); True }}}.
+  Proof.
+    (*@ func (gcoord *GroupCoordinator) SendUnprepare(rid, ts, rank uint64) {   @*)
+    (*@ }                                                                       @*)
+  Admitted.
+
+  Theorem wp_GroupCoordinator__SendQuery
+    (gcoord : loc) (rid : u64) (ts : u64) (rank : u64) gid γ :
+    is_gcoord gcoord gid γ -∗
+    {{{ True }}}
+      GroupCoordinator__SendQuery #gcoord #rid #ts #rank
+    {{{ RET #(); True }}}.
+  Proof.
+    (*@ func (gcoord *GroupCoordinator) SendQuery(rid, ts, rank uint64) {       @*)
+    (*@ }                                                                       @*)
+  Admitted.
+
+  Theorem wp_GroupCoordinator__SendRefresh
+    (gcoord : loc) (rid : u64) (ts : u64) (rank : u64) gid γ :
+    is_gcoord gcoord gid γ -∗
+    {{{ True }}}
+      GroupCoordinator__SendRefresh #gcoord #rid #ts #rank
+    {{{ RET #(); True }}}.
+  Proof.
+    (*@ func (gcoord *GroupCoordinator) SendRefresh(rid, ts, rank uint64) {     @*)
+    (*@ }                                                                       @*)
+  Admitted.
+
+  Theorem wp_GroupCoordinator__PrepareSession
+    (gcoord : loc) (rid : u64) (tsW : u64) (ptgsP : Slice.t) (pwrsP : loc) gid γ :
+    let ts := uint.nat tsW in
+    is_gcoord gcoord gid γ -∗
+    {{{ True }}}
+      GroupCoordinator__PrepareSession #gcoord #rid #tsW (to_val ptgsP) #pwrsP
+    {{{ RET #(); True }}}.
+  Proof.
+    iIntros (ts) "#Hgcoord".
+    iIntros (Φ) "!> _ HΦ".
+    wp_rec. wp_pures.
+
+    (*@ func (gcoord *GroupCoordinator) PrepareSession(rid uint64, ts uint64, ptgs []uint64, pwrs map[string]tulip.Value) { @*)
+    (*@     for {                                                               @*)
+    (*@                                                                         @*)
+    wp_apply (wp_forBreak (λ _, True)%I with "[] []"); last first; first 1 last.
+    { done. }
+    { clear Φ.
+
+      (*@         act, attached := gcoord.NextPrepareAction(rid, ts)              @*)
+      (*@                                                                         @*)
+      iIntros (Φ) "!> _ HΦ".
+      wp_apply (wp_GroupCoordinator__NextPrepareAction with "Hgcoord").
+      iIntros (action ok) "#Hsafea".
+      wp_pures.
+
+      (*@         if !attached {                                                  @*)
+      (*@             break                                                       @*)
+      (*@         }                                                               @*)
+      (*@                                                                         @*)
+      destruct ok; wp_pures; last by iApply "HΦ".
+
+      (*@         if act == GPP_FAST_PREPARE {                                    @*)
+      (*@             gcoord.SendFastPrepare(rid, ts, pwrs, ptgs)                 @*)
+      (*@         } else if act == GPP_VALIDATE {                                 @*)
+      (*@             gcoord.SendValidate(rid, ts, 1, pwrs, ptgs)                 @*)
+      (*@         } else if act == GPP_PREPARE {                                  @*)
+      (*@             gcoord.SendPrepare(rid, ts, 1)                              @*)
+      (*@         } else if act == GPP_UNPREPARE {                                @*)
+      (*@             gcoord.SendUnprepare(rid, ts, 1)                            @*)
+      (*@         } else if act == GPP_QUERY {                                    @*)
+      (*@             gcoord.SendQuery(rid, ts, 1)                                @*)
+      (*@         } else if act == GPP_REFRESH {                                  @*)
+      (*@             // Keep sending keep-alive message until the transaction terminated. @*)
+      (*@             gcoord.SendRefresh(rid, ts, 1)                              @*)
+      (*@         }                                                               @*)
+      (*@                                                                         @*)
+      (*@         if act == GPP_REFRESH {                                         @*)
+      (*@             primitive.Sleep(params.NS_SEND_REFRESH)                     @*)
+      (*@         } else {                                                        @*)
+      (*@             // The optimal time to sleep is the time required to arrive at a @*)
+      (*@             // prepare decision. Waking up too frequently means sending @*)
+      (*@             // unnecessary messages, too infrequently means longer latency when @*)
+      (*@             // messages are lost.                                       @*)
+      (*@             //                                                          @*)
+      (*@             // This might not be optimal for slow-path prepare. Consider @*)
+      (*@             // optimize this with CV wait and timeout.                  @*)
+      (*@             primitive.Sleep(params.NS_RESEND_PREPARE)                   @*)
+      (*@         }                                                               @*)
+      (*@     }                                                                   @*)
+      (*@                                                                         @*)
+      case_bool_decide as Hfp; wp_pures.
+      { wp_apply (wp_GroupCoordinator__SendFastPrepare with "Hgcoord").
+        wp_pures.
+        rewrite Hfp /=.
+        case_bool_decide; first done.
+        wp_apply wp_Sleep. wp_pures.
+        by iApply "HΦ".
+      }
+      case_bool_decide as Hvd; wp_pures.
+      { wp_apply (wp_GroupCoordinator__SendValidate with "Hgcoord").
+        wp_pures.
+        rewrite Hvd /=.
+        case_bool_decide; first done.
+        wp_apply wp_Sleep. wp_pures.
+        by iApply "HΦ".
+      }
+      case_bool_decide as Hprep; wp_pures.
+      { inv Hprep. destruct action; try done. simpl.
+        wp_apply (wp_GroupCoordinator__SendPrepare with "Hsafea Hgcoord").
+        wp_pures.
+        wp_apply wp_Sleep. wp_pures.
+        by iApply "HΦ".
+      }
+      case_bool_decide as Hunprep; wp_pures.
+      { inv Hunprep. destruct action; try done. simpl.
+        wp_apply (wp_GroupCoordinator__SendUnprepare with "Hsafea Hgcoord").
+        wp_pures.
+        wp_apply wp_Sleep. wp_pures.
+        by iApply "HΦ".
+      }
+      case_bool_decide as Hqr; wp_pures.
+      { wp_apply (wp_GroupCoordinator__SendQuery with "Hgcoord").
+        wp_pures.
+        rewrite Hqr /=.
+        case_bool_decide; first done.
+        wp_apply wp_Sleep. wp_pures.
+        by iApply "HΦ".
+      }
+      case_bool_decide as Hrf; wp_pures.
+      { wp_apply (wp_GroupCoordinator__SendRefresh with "Hgcoord").
+        wp_pures.
+        rewrite Hrf /=.
+        case_bool_decide; last done.
+        wp_apply wp_Sleep. wp_pures.
+        by iApply "HΦ".
+      }
+      case_bool_decide; first done.
+      wp_apply wp_Sleep. wp_pures.
+      by iApply "HΦ".
+
+      (*@     // The coordinator is no longer associated with @ts, this could happen only @*)
+      (*@     // after the prepare decision for @ts on @rid is made. Hence, this session @*)
+      (*@     // can terminate.                                                   @*)
+      (*@ }                                                                       @*)
+    }
+    wp_pures.
+    by iApply "HΦ".
+  Qed.
+
+  Theorem wp_GroupCoordinator__Prepare
+    (gcoord : loc) (tsW : u64) (ptgsP : Slice.t) (pwrsP : loc) gid γ :
+    let ts := uint.nat tsW in
+    is_gcoord gcoord gid γ -∗
+    {{{ True }}}
+      GroupCoordinator__Prepare #gcoord #tsW (to_val ptgsP) #pwrsP
+    {{{ (phase : txnphase) (valid : bool), RET (#(txnphase_to_u64 phase), #valid); 
+        if valid then safe_txnphase γ ts gid phase else True
+    }}}.
+  Proof.
+    iIntros (ts) "#Hgcoord".
+    iIntros (Φ) "!> _ HΦ".
+    wp_rec.
+
+    (*@ func (gcoord *GroupCoordinator) Prepare(ts uint64, ptgs []uint64, pwrs tulip.KVMap) (uint64, bool) { @*)
+    (*@     // Spawn a prepare session with each replica.                       @*)
+    (*@     for ridloop := range(gcoord.rps) {                                  @*)
+    (*@         rid := ridloop                                                  @*)
+    (*@         go func() {                                                     @*)
+    (*@             gcoord.PrepareSession(rid, ts, ptgs, pwrs)                  @*)
+    (*@         }()                                                             @*)
+    (*@     }                                                                   @*)
+    (*@                                                                         @*)
+    iPoseProof "Hgcoord" as "Hgcoord'".
+    do 2 iNamed "Hgcoord". iNamed "Hrps".
+    iRename "Hgcoord'" into "Hgcoord".
+    wp_loadField.
+    wp_apply (wp_MapIter_fold _ _ _ (λ _, True)%I with "Hrps []").
+    { done. }
+    { clear Φ.
+      iIntros (mx rid c Φ) "!> _ HΦ".
+      wp_pures.
+      wp_apply wp_fork.
+      { by wp_apply (wp_GroupCoordinator__PrepareSession with "Hgcoord"). }
+      by iApply "HΦ".
+    }
+    iIntros "_".
+
+    (*@     st, valid := gcoord.WaitUntilPrepareDone(ts)                        @*)
+    (*@     return st, valid                                                    @*)
+    (*@ }                                                                       @*)
+    wp_apply (wp_GroupCoordinator__WaitUntilPrepareDone with "Hgcoord").
+    iIntros (phase valid) "#Hsafep".
+    wp_pures.
+    by iApply "HΦ".
+  Qed.
+
+End program.
